---
title: "Lei_Zhuo_STAT425_HW5"
author: "Zhuo Feng Lei (zlei5)"
date: "1/28/2019"
output: pdf_document
---

## Question 1 

$$var(X^T_*\hat{\beta}) = X^T_*var(\hat{\beta})X_{*}$$

$$ = X^T_{*}(\sigma^2(X^TX)^{-1}X_*)$$

## Question 2

$$\hat{y} = X\hat{B} = X(X^TX)^{-1}X^TY = HY$$

$$var(\hat{y}) = H\sigma^2IH^T$$

$$ = H\sigma^2IH$$

$$ = \sigma^2H = \sigma^2X(X^TX)^{-1}X^T$$

## Question 3 

$$\hat{\epsilon} = Iy-X\hat{\beta}$$

$$ = X(X^TX)^{-1}X^Ty$$

$$ = y(I-X)(X^TX)^{-1}X^T$$

$$ = (XB+\epsilon)(I-X(X^TX)^{-1}X^T)$$

$$ = (I-X(X^TX)^{-1}X^T)\epsilon$$

## Question 4

$$HH = (X(X^TX)^{-1}X^T)(X(X^TX)^{-1}X^T)$$
     
$$ = X(X^TX)^{-1}(X^TX)(X^TX)^{-1}X^T$$
    
$$ = X(X^TX)^{-1}X^T$$
     
$$= H$$

$$H^T = [X(X^TX)^{-1}X^T]^{-1}$$
      
$$ = X[(X^TX)^{-1}]^TX^T$$
      
$$ = H$$
      
## Question 5

$$var(\epsilon) = \sigma^2I$$

$$\hat{\epsilon} = (I-H)\epsilon$$

$$var(\hat{\epsilon}) = \sigma^2(I-H)\sigma^2I(I-H)^T$$

$$= (I-H)\sigma^2I(I-H)$$

$$= \sigma^2(I-H)$$

$$var(\hat{\epsilon}) = \sigma^2(I-X(X^TX)^{-1}X^T)$$